theories/Data/SumN.v
@@ -1,80 +1,81 @@
+Require Import ExtLib.Data.POption.
 Require Import ExtLib.Data.Map.FMapPositive.
 Require Import ExtLib.Data.Eq.
 Require Import ExtLib.Tactics.Injection.
 
-Fixpoint pmap_lookup' (ts : pmap Type) (p : positive) : option Type :=
-  match p with
-    | xH => pmap_here ts
-    | xI p => pmap_lookup' (pmap_right ts) p
-    | xO p => pmap_lookup' (pmap_left ts) p
-  end.
+Set Universe Polymorphism.
 
-Record OneOf (ts : pmap Type) : Type := mkOneOf
+Section poly.
+  Polymorphic Universes Uv.
+
+Record OneOf (ts : pmap Type@{Uv}) : Type@{Uv} := mkOneOf
 { index : positive
-; value : match pmap_lookup' ts index with
-            | None => Empty_set
-            | Some T => T
+; value : match pmap_lookup_key ts index with
+          | pNone => Empty_set
+          | pSome T => T
           end
 }.
 
-Definition Into {ts} {T : Type} (n : positive) (pf : pmap_lookup' ts n = Some T)
+Definition Into {ts} {T : Type} (n : positive)
+           (pf : pmap_lookup_key ts n = pSome T)
 : T -> OneOf ts :=
   match pf in _ = X return match X with
-                           | Some T => T
-                           | None => Empty_set
+                           | pSome T => T
+                           | pNone => Empty_set
                            end -> OneOf ts
   with
   | eq_refl => @mkOneOf ts n
   end.
 
 Fixpoint asNth' {ts : pmap Type} (p p' : positive)
-: match pmap_lookup' ts p' with
-    | None => Empty_set
-    | Some T => T
-  end -> option (match pmap_lookup' ts p with
-                   | None => Empty_set
-                   | Some T => T
+: match pmap_lookup_key ts p' with
+    | pNone => Empty_set
+    | pSome T => T
+  end -> poption (match pmap_lookup_key ts p with
+                   | pNone => Empty_set
+                   | pSome T => T
                  end) :=
   match p as p , p' as p'
-        return match pmap_lookup' ts p' with
-                 | None => Empty_set
-                 | Some T => T
-               end -> option (match pmap_lookup' ts p with
-                                | None => Empty_set
-                                | Some T => T
-                              end)
+        return match pmap_lookup_key ts p' with
+                 | pNone => Empty_set
+                 | pSome T => T
+               end -> poption (match pmap_lookup_key ts p with
+                               | pNone => Empty_set
+                               | pSome T => T
+                               end)
   with
-    | xH , xH => Some
+    | xH , xH => pSome
     | xI p , xI p' => asNth' p p'
     | xO p , xO p' => asNth' p p'
-    | _ , _ => fun _ => None
+    | _ , _ => fun _ => pNone
   end.
 
 Definition asNth {ts : pmap Type} (p : positive) (oe : OneOf ts)
-: option (match pmap_lookup' ts p with
-            | None => Empty_set
-            | Some T => T
+: poption (match pmap_lookup_key ts p with
+          | pNone => Empty_set
+          | pSome T => T
           end) :=
   @asNth' ts p oe.(index ts) oe.(value ts).
 
 Definition OutOf {ts} {T : Type} (n : positive)
-           (pf : pmap_lookup' ts n = Some T)
-: OneOf ts -> option T :=
-  match pf in _ = X return OneOf ts -> option match X with
-                                              | None => Empty_set:Type
-                                              | Some T => T
-                                              end
+           (pf : pmap_lookup_key ts n = pSome T)
+: OneOf ts -> poption T :=
+  match pf in _ = X
+        return OneOf ts -> poption match X return Type@{Uv} with
+                                   | pNone => Empty_set
+                                   | pSome T => T
+                                   end
   with
   | eq_refl => @asNth ts n
   end.
 
-Lemma asNth'_get_lookup : forall p ts v, asNth' (ts:=ts) p p v = Some v.
+Lemma asNth'_get_lookup : forall p ts v, asNth' (ts:=ts) p p v = pSome v.
 Proof.
   induction p; simpl; intros; auto.
 Qed.
 
 Theorem Outof_Into : forall ts T p pf v,
-    @OutOf ts T p pf (@Into ts T p pf v) = Some v.
+    @OutOf ts T p pf (@Into ts T p pf v) = pSome v.
 Proof using.
   unfold OutOf, Into.
   intros.
@@ -83,13 +84,13 @@ Proof using.
   repeat rewrite (eq_Const_eq (eq_sym pf)).
   unfold asNth. simpl.
   rewrite asNth'_get_lookup.
-  { generalize dependent (pmap_lookup' ts p).
+  { generalize dependent (pmap_lookup_key ts p).
     intros. subst. reflexivity. }
 Qed.
 
 Theorem asNth_eq
 : forall ts p oe v,
-    @asNth ts p oe = Some v ->
+    @asNth ts p oe = pSome v ->
     oe = {| index := p ; value := v |}.
 Proof.
   unfold asNth.
@@ -105,42 +106,28 @@ Section elim.
 
   Fixpoint pmap_elim (R : Type) (ts : pmap T) : Type :=
     match ts with
-      | Empty => R
-      | Branch None l r => pmap_elim (pmap_elim R r) l
-      | Branch (Some x) l r => F x -> pmap_elim (pmap_elim R r) l
+    | Empty => R
+    | Branch pNone l r => pmap_elim (pmap_elim R r) l
+    | Branch (pSome x) l r => F x -> pmap_elim (pmap_elim R r) l
     end.
 End elim.
 
-Fixpoint pmap_lookup'_Empty (p : positive) : pmap_lookup' Empty p = None :=
-  match p with
-    | xH => eq_refl
-    | xO p => pmap_lookup'_Empty p
-    | xI p => pmap_lookup'_Empty p
-  end.
-
 Definition OneOf_Empty (f : OneOf Empty) : False.
 Proof.
-  destruct f. rewrite pmap_lookup'_Empty in *.
+  destruct f. rewrite pmap_lookup_key_Empty in *.
   intuition congruence.
 Defined.
 
-Lemma pmap_lookup'_eq p m : pmap_lookup p m = pmap_lookup' m p.
-Proof.
-  generalize dependent m. induction p; intuition.
-  simpl. destruct m. simpl. rewrite pmap_lookup'_Empty. reflexivity.
-  simpl in *. apply IHp.
-  simpl in *. destruct m. simpl. rewrite pmap_lookup'_Empty. reflexivity.
-  simpl. apply IHp.
-Defined.
+
 
 Global Instance Injective_OneOf m i1 i2 v1 v2
 : Injective (@eq (OneOf m)
                  {| index := i1 ; value := v1 |}
                  {| index := i2 ; value := v2 |}) :=
 { result := exists pf : i2 = i1,
-    v1 = match pf in _ = T return match pmap_lookup' m T with
-                                  | None => Empty_set
-                                  | Some T => T
+    v1 = match pf in _ = T return match pmap_lookup_key m T return Type@{Uv} with
+                                  | pNone => Empty_set
+                                  | pSome T => T
                                   end with
          | eq_refl => v2
          end
@@ -151,9 +138,9 @@ Global Instance Injective_OneOf m i1 i2 v1 v2
           v1 = match
             pf in (_ = T)
             return
-            match pmap_lookup' m T with
-            | Some T0 => T0
-            | None => Empty_set
+            match pmap_lookup_key m T return Type@{Uv} with
+            | pSome T0 => T0
+            | pNone => Empty_set
             end
           with
           | eq_refl => value _ h
@@ -162,3 +149,5 @@ Global Instance Injective_OneOf m i1 i2 v1 v2
       | eq_refl => @ex_intro _ _ eq_refl eq_refl
       end
 }.
+
+End poly.
